Pedro-Coq/proofs/CogActionExecution.v
@@ -1,0 +1,402 @@
+From Coq Require Import Lia List ZArith.
+From compcert Require Import Archi AST Clight Clightdefs ClightBigstep Cop Ctypes
+  Errors Events Floats Globalenvs Integers Maps Memory Values.
+From Pedro.Generated Require Import us_mario jp_mario.
+From Pedro.Proofs Require Import GameTypes TTCCogExecution SlideKickDustExecution.
+Import ListNotations.
+Open Scope Z_scope.
+Module CA := us_mario.
+
+Definition cog_floor_class_function version : function :=
+  match version with VersionUS => CA.f_mario_get_floor_class
+                   | VersionJP => jp_mario.f_mario_get_floor_class end.
+Definition cog_moving_transition_function version : function :=
+  match version with VersionUS => CA.f_set_mario_action_moving
+                   | VersionJP => jp_mario.f_set_mario_action_moving end.
+Definition cog_terrain_function version : function :=
+  match version with VersionUS => CA.f_mario_get_terrain_sound_addend
+                   | VersionJP => jp_mario.f_mario_get_terrain_sound_addend end.
+
+Record cog_action_layout (ge : Clight.genv) (caller : slide_caller_layout ge) : Type := {
+  action_area_co : composite;
+  action_surface_co : composite;
+  action_area_lookup : (genv_cenv ge) ! CA._Area = Some action_area_co;
+  action_surface_lookup : (genv_cenv ge) ! CA._Surface = Some action_surface_co;
+  action_area_offset : field_offset (genv_cenv ge) CA._area
+    (co_members (slide_mario_co ge caller)) = OK (144, Full);
+  action_flags_offset : field_offset (genv_cenv ge) CA._flags
+    (co_members (slide_mario_co ge caller)) = OK (4, Full);
+  action_action_offset : field_offset (genv_cenv ge) CA._action
+    (co_members (slide_mario_co ge caller)) = OK (12, Full);
+  action_prev_offset : field_offset (genv_cenv ge) CA._prevAction
+    (co_members (slide_mario_co ge caller)) = OK (16, Full);
+  action_state_offset : field_offset (genv_cenv ge) CA._actionState
+    (co_members (slide_mario_co ge caller)) = OK (24, Full);
+  action_timer_offset : field_offset (genv_cenv ge) CA._actionTimer
+    (co_members (slide_mario_co ge caller)) = OK (26, Full);
+  action_arg_offset : field_offset (genv_cenv ge) CA._actionArg
+    (co_members (slide_mario_co ge caller)) = OK (28, Full);
+  action_mag_offset : field_offset (genv_cenv ge) CA._intendedMag
+    (co_members (slide_mario_co ge caller)) = OK (32, Full);
+  action_speed_offset : field_offset (genv_cenv ge) CA._forwardVel
+    (co_members (slide_mario_co ge caller)) = OK (84, Full);
+  action_water_offset : field_offset (genv_cenv ge) CA._waterLevel
+    (co_members (slide_mario_co ge caller)) = OK (118, Full);
+  action_terrain_type_offset : field_offset (genv_cenv ge) CA._terrainType
+    (co_members action_area_co) = OK (2, Full);
+  action_surface_type_offset : field_offset (genv_cenv ge) CA._type
+    (co_members action_surface_co) = OK (0, Full)
+}.
+
+(** Ordinary TTC terrain and retained default floor. This is an entry memory
+    image, not a reachability or collision-selection assertion. *)
+Definition cog_default_floor_image memory mario area floor : Prop :=
+  Mem.load Mptr memory mario 144 = Some (Vptr area Ptrofs.zero) /\
+  Mem.load Mint16unsigned memory area 2 = Some (Vint Int.one) /\
+  Mem.load Mptr memory mario 104 = Some (Vptr floor Ptrofs.zero) /\
+  Mem.load Mint16signed memory floor 0 = Some (Vint Int.zero) /\
+  Mem.load Mint32 memory mario 12 = Some (Vint (Int.repr 8389722)).
+
+Lemma cog_readable_floor_is_valid : forall memory floor value,
+  Mem.load Mint16signed memory floor 0 = Some value ->
+  Mem.weak_valid_pointer memory floor 0 = true.
+Proof.
+  intros memory floor value Hload.
+  pose proof (Mem.load_valid_access _ _ _ _ _ Hload) as [Hrange Halign].
+  apply Mem.valid_pointer_implies. apply Mem.valid_pointer_nonempty_perm.
+  eapply Mem.perm_implies; [apply Hrange; cbn; lia | constructor].
+Qed.
+
+Lemma cog_surface_nonnull : forall ce memory b,
+  Mem.weak_valid_pointer memory b 0 = true ->
+  sem_binary_operation ce One (Vptr b Ptrofs.zero)
+    (tptr (Tstruct CA._Surface noattr)) (Vint Int.zero) (tptr tvoid) memory =
+    Some (Vint Int.one).
+Proof.
+  intros ce memory b Hvalid.
+  assert (H32 : Archi.ptr64 = false) by reflexivity.
+  assert (Hzero : Ptrofs.unsigned Ptrofs.zero = 0) by reflexivity.
+  cbn. unfold cmp_ptr. rewrite H32. cbn [Val.cmpu_bool].
+  rewrite H32, Int.eq_true. cbn.
+  rewrite Hzero. fold (Mem.weak_valid_pointer memory b 0).
+  rewrite Hvalid. reflexivity.
+Qed.
+
+Lemma cog_dry_floor_comparison : forall ce memory height water,
+  Float32.cmp Clt height (Float32.of_int (Int.sub water (Int.repr 10))) = false ->
+  sem_binary_operation ce Olt (Vsingle height) tfloat
+    (Vint (Int.sub water (Int.repr 10))) tint memory = Some (Vint Int.zero).
+Proof.
+  intros ce memory height water Hdry.
+  change (Some (Val.of_bool
+    (Float32.cmp Clt height (Float32.of_int (Int.sub water (Int.repr 10))))) =
+    Some (Vint Int.zero)).
+  rewrite Hdry. reflexivity.
+Qed.
+
+Ltac action_normalize :=
+  first [solve [eapply cog_surface_nonnull; eassumption] |
+    solve [eapply cog_dry_floor_comparison; eassumption] |
+    solve [cbn; reflexivity] |
+    match goal with |- ?G => idtac "ACTION OPERATION" G end; fail 100].
+Ltac action_check tac :=
+  first [solve [tac] | match goal with |- ?G => idtac "ACTION ATOMIC" G end; fail 100].
+Ltac action_expr :=
+  lazymatch goal with
+  | |- eval_expr _ _ _ _ (Econst_int _ _) _ => constructor
+  | |- eval_expr _ _ _ _ (Econst_single _ _) _ => constructor
+  | |- eval_expr _ _ _ _ (Etempvar _ _) _ => eapply eval_Etempvar; cbn; reflexivity
+  | |- eval_expr _ _ _ _ (Ebinop _ _ _ _) _ =>
+      eapply eval_Ebinop; [action_expr | action_expr | action_normalize]
+  | |- eval_expr _ _ _ _ (Eunop _ _ _) _ =>
+      eapply eval_Eunop; [action_expr | action_normalize]
+  | |- eval_expr _ _ _ _ (Ecast _ _) _ =>
+      eapply eval_Ecast; [action_expr | action_normalize]
+  | |- eval_expr _ _ _ _ _ _ =>
+      eapply eval_Elvalue; [action_lvalue |
+       first [eapply deref_loc_value; [reflexivity | cbn; action_check cog_memory_load]
+             |eapply deref_loc_reference; reflexivity
+             |eapply deref_loc_copy; reflexivity]]
+  end
+with action_lvalue :=
+  lazymatch goal with
+  | |- eval_lvalue _ _ _ _ (Evar _ _) _ _ _ =>
+      eapply eval_Evar_global; [reflexivity | eassumption]
+  | |- eval_lvalue _ _ _ _ (Ederef _ _) _ _ _ => eapply eval_Ederef; action_expr
+  | |- eval_lvalue _ _ _ _ (Efield _ _ _) _ _ _ =>
+      eapply eval_Efield_struct; [action_expr | reflexivity | eassumption | eassumption]
+  end.
+Ltac action_arguments :=
+  first [apply eval_Enil |
+    eapply eval_Econs; [action_expr | cbn; reflexivity | action_arguments]].
+Ltac action_stmt :=
+  lazymatch goal with
+  | |- exec_stmt _ _ _ _ _ Sskip _ _ _ _ => constructor
+  | |- exec_stmt _ _ _ _ _ Sbreak _ _ _ _ => constructor
+  | |- exec_stmt _ _ _ _ _ (Ssequence _ _) _ _ _ _ =>
+      first [eapply exec_Sseq_1 with (t1 := E0) (t2 := E0); [action_stmt | action_stmt]
+            |eapply exec_Sseq_2; [action_stmt | discriminate]]
+  | |- exec_stmt _ _ _ _ _ (Sset _ _) _ _ _ _ => eapply exec_Sset; action_expr
+  | |- exec_stmt _ _ _ _ _ (Sassign _ _) _ _ _ _ =>
+      eapply exec_Sassign;
+      [action_lvalue | action_expr | cbn; reflexivity |
+       eapply assign_loc_value; [reflexivity | cbn; eassumption]]
+  | |- exec_stmt _ _ _ _ _ (Sifthenelse _ _ _) _ _ _ _ =>
+      eapply exec_Sifthenelse;
+      [action_expr | action_check ltac:(cbn; reflexivity) | cog_reduce_statement; action_stmt]
+  | |- exec_stmt _ _ _ _ _ (Sswitch _ _) _ _ _ _ =>
+      first [eapply exec_Sswitch with (out := Out_normal);
+        [action_expr | cbn; reflexivity | cog_reduce_statement; action_stmt] |
+        eapply exec_Sswitch with (out := Out_break);
+        [action_expr | cbn; reflexivity | cog_reduce_statement; action_stmt]]
+  | |- exec_stmt _ _ _ _ _ (Sreturn (Some _)) _ _ _ _ =>
+      eapply exec_Sreturn_some; action_expr
+  | |- exec_stmt _ _ _ _ _ (Scall _ _ _) _ _ _ _ =>
+      eapply exec_Scall;
+      [reflexivity | action_expr | action_arguments |
+       eapply cog_find_funct_zero; eassumption | reflexivity | eassumption]
+  end.
+Ltac action_entry :=
+  eapply function_entry2_intro;
+  [cbn; apply Coqlib.list_norepet_nil | cbn; cog_norepet |
+   vm_compute; intros x y Hx Hy Heq; subst y; intuition congruence |
+   cbn; apply alloc_variables_nil | cbn; reflexivity].
+
+Theorem generated_cog_default_floor_class_us_jp :
+  forall version ge memory mario area floor (caller : slide_caller_layout ge),
+    cog_action_layout ge caller ->
+    cog_default_floor_image memory mario area floor ->
+    eval_funcall function_entry2 ge memory (Internal (cog_floor_class_function version))
+      [Vptr mario Ptrofs.zero] E0 memory (Vint Int.zero).
+Proof.
+  intros version ge memory mario area floor caller Hlayout Himage.
+  destruct Hlayout; destruct caller; cbn in *.
+  destruct Himage as [Ha [Ht [Hf [Hft Hact]]]].
+  pose proof (cog_readable_floor_is_valid _ _ _ Hft) as Hvalid.
+  destruct version; cbn [cog_floor_class_function]; eapply eval_funcall_internal;
+    [action_entry | simpl fn_body; timeout 10 action_stmt |
+     cbn; split; [discriminate | reflexivity] | cbn; reflexivity |
+     action_entry | simpl fn_body; timeout 10 action_stmt |
+     cbn; split; [discriminate | reflexivity] | cbn; reflexivity].
+Qed.
+
+Theorem generated_cog_moving_kb_transition_us_jp :
+  forall version ge memory mario area floor speed floor_code (caller : slide_caller_layout ge),
+    cog_action_layout ge caller ->
+    cog_default_floor_image memory mario area floor ->
+    Mem.load Mfloat32 memory mario 84 = Some (Vsingle speed) ->
+    Mem.load Mfloat32 memory mario 32 = Some (Vsingle Float32.zero) ->
+    Genv.find_symbol ge CA._mario_get_floor_class = Some floor_code ->
+    Genv.find_funct_ptr ge floor_code = Some (Internal (cog_floor_class_function version)) ->
+    eval_funcall function_entry2 ge memory (Internal (cog_moving_transition_function version))
+      [Vptr mario Ptrofs.zero; Vint (Int.repr 132194); Vint Int.zero]
+      E0 memory (Vint (Int.repr 132194)).
+Proof.
+  intros version ge memory mario area floor speed floor_code caller Hlayout Himage
+    Hspeed Hmag Hsymbol Hcode.
+  pose proof (generated_cog_default_floor_class_us_jp version ge memory mario area floor
+    caller Hlayout Himage) as Hfloor.
+  destruct Hlayout; destruct caller; cbn in *.
+  destruct version; cbn [cog_moving_transition_function]; eapply eval_funcall_internal;
+    [action_entry | simpl fn_body; timeout 10 action_stmt |
+     cbn; split; [discriminate | reflexivity] | cbn; reflexivity |
+     action_entry | simpl fn_body; timeout 10 action_stmt |
+     cbn; split; [discriminate | reflexivity] | cbn; reflexivity].
+Qed.
+
+Definition kb_sound_flags flags : int :=
+  Int.and flags (Int.not (Int.or (Int.repr 65536) (Int.repr 131072))).
+Definition kb_entry_flags flags : int :=
+  Int.and (kb_sound_flags flags) (Int.not (Int.repr 262144)).
+
+Definition cog_kb_transition_stores before m1 m2 m3 m4 m5 m6 after mario flags : Prop :=
+  Mem.store Mint32 before mario 4 (Vint (kb_sound_flags flags)) = Some m1 /\
+  Mem.store Mint32 m1 mario 4 (Vint (kb_entry_flags flags)) = Some m2 /\
+  Mem.store Mint32 m2 mario 16 (Vint (Int.repr 8389722)) = Some m3 /\
+  Mem.store Mint32 m3 mario 12 (Vint (Int.repr 132194)) = Some m4 /\
+  Mem.store Mint32 m4 mario 28 (Vint Int.zero) = Some m5 /\
+  Mem.store Mint16unsigned m5 mario 24 (Vint Int.zero) = Some m6 /\
+  Mem.store Mint16unsigned m6 mario 26 (Vint Int.zero) = Some after.
+
+Definition cog_kb_writable memory mario : Prop :=
+  Mem.valid_access memory Mint32 mario 4 Writable /\
+  Mem.valid_access memory Mint32 mario 16 Writable /\
+  Mem.valid_access memory Mint32 mario 12 Writable /\
+  Mem.valid_access memory Mint32 mario 28 Writable /\
+  Mem.valid_access memory Mint16unsigned mario 24 Writable /\
+  Mem.valid_access memory Mint16unsigned mario 26 Writable.
+
+(** Executes both real nested helpers and all seven stores of set_mario_action.
+    Neither a callee execution nor a position/floor preservation equation is
+    an input to this theorem. *)
+Theorem generated_cog_kb_transition_with_stores_us_jp :
+  forall version ge before m1 m2 m3 m4 m5 m6 after mario area floor speed flags
+      floor_code moving_code (caller : slide_caller_layout ge),
+    cog_action_layout ge caller ->
+    cog_default_floor_image before mario area floor ->
+    Mem.load Mfloat32 before mario 84 = Some (Vsingle speed) ->
+    Mem.load Mfloat32 before mario 32 = Some (Vsingle Float32.zero) ->
+    Mem.load Mint32 before mario 4 = Some (Vint flags) ->
+    Genv.find_symbol ge CA._mario_get_floor_class = Some floor_code ->
+    Genv.find_funct_ptr ge floor_code = Some (Internal (cog_floor_class_function version)) ->
+    Genv.find_symbol ge CA._set_mario_action_moving = Some moving_code ->
+    Genv.find_funct_ptr ge moving_code = Some (Internal (cog_moving_transition_function version)) ->
+    cog_kb_transition_stores before m1 m2 m3 m4 m5 m6 after mario flags ->
+    eval_funcall function_entry2 ge before (Internal (slide_action_function version))
+      [Vptr mario Ptrofs.zero; Vint (Int.repr 132194); Vint Int.zero]
+      E0 after (Vint Int.one).
+Proof.
+  intros version ge before m1 m2 m3 m4 m5 m6 after mario area floor speed flags
+    floor_code moving_code caller Hlayout Himage Hspeed Hmag Hflags Hfloor_symbol Hfloor_code
+    Hmoving_symbol Hmoving_code Hstores.
+  pose proof (generated_cog_moving_kb_transition_us_jp version ge before mario area floor
+    speed floor_code caller Hlayout Himage Hspeed Hmag Hfloor_symbol Hfloor_code) as Hmoving.
+  destruct Himage as [Ha [Ht [Hf [Hft Hact]]]].
+  destruct Hstores as [Hs1 [Hs2 [Hs3 [Hs4 [Hs5 [Hs6 Hs7]]]]]].
+  destruct Hlayout; destruct caller; cbn in *.
+  destruct version; cbn [slide_action_function]; eapply eval_funcall_internal;
+    [action_entry | simpl fn_body; timeout 15 action_stmt |
+     cbn; split; [discriminate | reflexivity] | cbn; reflexivity |
+     action_entry | simpl fn_body; timeout 15 action_stmt |
+     cbn; split; [discriminate | reflexivity] | cbn; reflexivity].
+Qed.
+
+Definition cog_kb_untouched (mario b : block) chunk offset : Prop :=
+  b <> mario \/ offset + size_chunk chunk <= 4 \/ 32 <= offset \/
+  (8 <= offset /\ offset + size_chunk chunk <= 12) \/
+  (20 <= offset /\ offset + size_chunk chunk <= 24).
+
+Lemma cog_kb_transition_frame :
+  forall before m1 m2 m3 m4 m5 m6 after mario flags,
+    cog_kb_transition_stores before m1 m2 m3 m4 m5 m6 after mario flags ->
+    forall chunk b offset, cog_kb_untouched mario b chunk offset ->
+      Mem.load chunk after b offset = Mem.load chunk before b offset.
+Proof.
+  intros before m1 m2 m3 m4 m5 m6 after mario flags
+    [Hs1 [Hs2 [Hs3 [Hs4 [Hs5 [Hs6 Hs7]]]]]] chunk b offset Hsafe.
+  unfold cog_kb_untouched in Hsafe.
+  repeat match goal with
+  | H : Mem.store _ _ _ _ _ = Some ?out |- Mem.load _ ?out _ _ = _ =>
+      rewrite (Mem.load_store_other _ _ _ _ _ _ H) by (cbn; intuition lia)
+  end. reflexivity.
+Qed.
+
+Lemma cog_kb_transition_anchor :
+  forall before m1 m2 m3 m4 m5 m6 after mario flags,
+    cog_kb_transition_stores before m1 m2 m3 m4 m5 m6 after mario flags ->
+    slide_anchor after mario = slide_anchor before mario.
+Proof.
+  intros before m1 m2 m3 m4 m5 m6 after mario flags Hstores.
+  unfold slide_anchor.
+  repeat rewrite (cog_kb_transition_frame _ _ _ _ _ _ _ _ _ _ Hstores)
+    by (unfold cog_kb_untouched; cbn; intuition lia).
+  reflexivity.
+Qed.
+
+Theorem generated_cog_kb_transition_executes_and_frames_us_jp :
+  forall version ge before mario area floor speed flags floor_code moving_code
+      (caller : slide_caller_layout ge),
+    cog_action_layout ge caller ->
+    cog_default_floor_image before mario area floor ->
+    Mem.load Mfloat32 before mario 84 = Some (Vsingle speed) ->
+    Mem.load Mfloat32 before mario 32 = Some (Vsingle Float32.zero) ->
+    Mem.load Mint32 before mario 4 = Some (Vint flags) ->
+    cog_kb_writable before mario ->
+    Genv.find_symbol ge CA._mario_get_floor_class = Some floor_code ->
+    Genv.find_funct_ptr ge floor_code = Some (Internal (cog_floor_class_function version)) ->
+    Genv.find_symbol ge CA._set_mario_action_moving = Some moving_code ->
+    Genv.find_funct_ptr ge moving_code = Some (Internal (cog_moving_transition_function version)) ->
+    exists m1 m2 m3 m4 m5 m6 after,
+      cog_kb_transition_stores before m1 m2 m3 m4 m5 m6 after mario flags /\
+      eval_funcall function_entry2 ge before (Internal (slide_action_function version))
+        [Vptr mario Ptrofs.zero; Vint (Int.repr 132194); Vint Int.zero]
+        E0 after (Vint Int.one) /\
+      slide_anchor after mario = slide_anchor before mario /\
+      Mem.load Mint32 after mario 12 = Some (Vint (Int.repr 132194)) /\
+      Mem.load Mint32 after mario 16 = Some (Vint (Int.repr 8389722)) /\
+      Mem.load Mint32 after mario 28 = Some (Vint Int.zero) /\
+      Mem.load Mint16unsigned after mario 24 = Some (Vint Int.zero) /\
+      Mem.load Mint16unsigned after mario 26 = Some (Vint Int.zero) /\
+      (forall chunk b offset, cog_kb_untouched mario b chunk offset ->
+        Mem.load chunk after b offset = Mem.load chunk before b offset).
+Proof.
+  intros version ge before mario area floor speed flags floor_code moving_code caller
+    Hlayout Himage Hspeed Hmag Hflags Hwrite Hfs Hfc Hms Hmc.
+  destruct Hwrite as [Hw1 [Hw2 [Hw3 [Hw4 [Hw5 Hw6]]]]].
+  destruct (Mem.valid_access_store before Mint32 mario 4 (Vint (kb_sound_flags flags))
+    ltac:(cog_memory_access)) as [m1 Hs1].
+  destruct (Mem.valid_access_store m1 Mint32 mario 4 (Vint (kb_entry_flags flags))
+    ltac:(cog_memory_access)) as [m2 Hs2].
+  destruct (Mem.valid_access_store m2 Mint32 mario 16 (Vint (Int.repr 8389722))
+    ltac:(cog_memory_access)) as [m3 Hs3].
+  destruct (Mem.valid_access_store m3 Mint32 mario 12 (Vint (Int.repr 132194))
+    ltac:(cog_memory_access)) as [m4 Hs4].
+  destruct (Mem.valid_access_store m4 Mint32 mario 28 (Vint Int.zero)
+    ltac:(cog_memory_access)) as [m5 Hs5].
+  destruct (Mem.valid_access_store m5 Mint16unsigned mario 24 (Vint Int.zero)
+    ltac:(cog_memory_access)) as [m6 Hs6].
+  destruct (Mem.valid_access_store m6 Mint16unsigned mario 26 (Vint Int.zero)
+    ltac:(cog_memory_access)) as [after Hs7].
+  assert (Hstores : cog_kb_transition_stores before m1 m2 m3 m4 m5 m6 after mario flags)
+    by (repeat split; assumption).
+  exists m1, m2, m3, m4, m5, m6, after. split; [exact Hstores |].
+  split; [eapply generated_cog_kb_transition_with_stores_us_jp; eassumption |].
+  split; [eapply cog_kb_transition_anchor; eassumption |].
+  repeat apply conj; try solve [cog_memory_load].
+  exact (cog_kb_transition_frame _ _ _ _ _ _ _ _ _ _ Hstores).
+Qed.
+
+(** Dry TTC/default-floor branch: TERRAIN_STONE is terrain row 1, but the
+    row's default sound is SOUND_TERRAIN_STONE = 3, not 0 or 1. *)
+Definition cog_terrain_execution_claim version : Prop :=
+  forall ge memory mario area floor level table height water
+      (caller : slide_caller_layout ge),
+    cog_action_layout ge caller ->
+    cog_default_floor_image memory mario area floor ->
+    Genv.find_symbol ge CA._gCurrLevelNum = Some level ->
+    Genv.find_symbol ge CA._sTerrainSounds = Some table ->
+    Mem.load Mint16signed memory level 0 = Some (Vint (Int.repr 14)) ->
+    Mem.load Mfloat32 memory mario 112 = Some (Vsingle height) ->
+    Mem.load Mint16signed memory mario 118 = Some (Vint water) ->
+    Float32.cmp Clt height (Float32.of_int (Int.sub water (Int.repr 10))) = false ->
+    Mem.load Mint8signed memory table 6 = Some (Vint (Int.repr 3)) ->
+    eval_funcall function_entry2 ge memory (Internal (cog_terrain_function version))
+      [Vptr mario Ptrofs.zero] E0 memory (Vint (Int.repr 196608)).
+
+Theorem generated_cog_stone_terrain_addend_us_jp :
+  forall version, cog_terrain_execution_claim version.
+Proof.
+  intros version ge memory mario area floor level table height water caller Hlayout
+    Himage Hlevel Htable Hlevel_load Hheight Hwater Hdry Hsound.
+  destruct Himage as [Ha [Ht [Hf [Hft Hact]]]].
+  pose proof (cog_readable_floor_is_valid _ _ _ Hft) as Hvalid.
+  destruct Hlayout; destruct caller; cbn in *.
+  destruct version; cbn [cog_terrain_function]; eapply eval_funcall_internal;
+    [action_entry | simpl fn_body; timeout 15 action_stmt |
+     cbn; split; [discriminate | reflexivity] | cbn; reflexivity |
+     action_entry | simpl fn_body; timeout 15 action_stmt |
+     cbn; split; [discriminate | reflexivity] | cbn; reflexivity].
+Qed.
+
+Definition cog_action_layout_offsets version :=
+  let ce := prog_comp_env
+    (match version with VersionUS => CA.prog | VersionJP => jp_mario.prog end) in
+  map (fun item => field_offset ce (snd item)
+    (match ce ! (fst item) with Some co => co_members co | None => [] end))
+    [(CA._MarioState,CA._area); (CA._MarioState,CA._flags);
+     (CA._MarioState,CA._action); (CA._MarioState,CA._prevAction);
+     (CA._MarioState,CA._actionState); (CA._MarioState,CA._actionTimer);
+     (CA._MarioState,CA._actionArg); (CA._MarioState,CA._intendedMag);
+     (CA._MarioState,CA._forwardVel); (CA._MarioState,CA._waterLevel);
+     (CA._Area,CA._terrainType); (CA._Surface,CA._type)].
+
+Definition cog_action_layout_receipt : Prop :=
+  (forall version, cog_action_layout_offsets version =
+    map (fun offset => OK (offset, Full)) [144;4;12;16;24;26;28;32;84;118;2;0]) /\
+  nth_error (gvar_init CA.v_sTerrainSounds) 6 = Some (Init_int8 (Int.repr 3)) /\
+  nth_error (gvar_init jp_mario.v_sTerrainSounds) 6 = Some (Init_int8 (Int.repr 3)).
+
+Theorem cog_action_layout_generated_us_jp : cog_action_layout_receipt.
+Proof.
+  split; [intros []; vm_compute; reflexivity | split; reflexivity].
+Qed.
